testdata/cue/comprehensions/guard_incomplete_defers.cue
@@ -1,0 +1,6 @@
+x: bool
+out: {
+	if x {
+		a: 1
+	}
+}
